\documentclass[10pt, AMS Euler]{article}
\textheight=9.25in \textwidth=7in \topmargin=-.75in
 \oddsidemargin=-0.25in
\evensidemargin=-0.25in
\usepackage{url}  % The bib file uses this
\usepackage{graphicx} %to import pictures
\usepackage{amsmath, amssymb}
\usepackage{theorem, multicol, color}
\usepackage{gfsartemisia-euler}


\setlength{\intextsep}{5mm} \setlength{\textfloatsep}{5mm}
\setlength{\floatsep}{5mm}
\setlength{\parindent}{0em} % new paragraphs are not indented


%%%%  SHORTCUT COMMANDS  %%%%
\newcommand{\ds}{\displaystyle}
\newcommand{\Z}{\mathbb{Z}}
\newcommand{\arc}{\rightarrow}
\newcommand{\R}{\mathbb{R}}
\newcommand{\N}{\mathbb{N}}
\newcommand{\Q}{\mathbb{Q}}
\newcommand{\blank}{\underline{\hspace{0.33in}}}
\newcommand{\qand}{\quad and \quad}
\renewcommand{\stirling}[2]{\genfrac{\{}{\}}{0pt}{}{#1}{#2}}
\newcommand{\dydx}{\ds \frac{d y}{d x}}
\newcommand{\ddx}{\ds \frac{d}{d x}}
\newcommand{\dvdx}{\ds \frac{d v}{d x}} 

%%%%  footnote style %%%%

\renewcommand{\thefootnote}{\fnsymbol{footnote}}

\pagestyle{empty}

\begin{document}

\begin{flushright}
Chandler Justice - A02313187
\end{flushright}
\noindent \underline{\hspace{3in}}\\

\textbf{January 10, 2024}\\

\textbf{Example:} We assume that $f$ has a derivative at $x = a$.

$f'(a) = \lim_{x\to\infty} \frac{f(x) - f(a)}{x - a} \approx \frac{f(x) - f(a)}{x - a}, x \neq a$\\

We can also say $x = a + h$ and we get $f'(a) = \lim_{h \to 0} \frac{f(a + h) - f(a)}{h} \approx \frac{f(a + h) - f(a)}{h}$\\

\textit{Note:} in the textbook, they may refer to $a$ as $\bar{x}$\\

We can then construct the equation $D_+ f(\bar{x}) = \frac{f(\bar{x} + h) - f(\bar{x})}{h}, h \geq h_0 \geq 0$\\

\textbf{Example:} Maltheas Population Model\\

\[ 
    \begin{cases}
        \frac{dA}{dt} = kA\\
        A(0) = A_0\\
    \end{cases}\\
\]    
\[    
    \frac{dA}{dt} \approx \frac{A(t + h) - A(t)}{h}\\
\]
\[
    A'(t) \approx D_+ A(t)\\
\]   
    \[   
    \begin{cases}
        \frac{A(t + h) - A(t)}{h} \approx kA(t^*)\\
        A(0) = A_0
    \end{cases}\\
\] 
\[   
    h = \Delta t\\
\]    
\[
    \frac{A(t + \Delta t) - A(t)}{h} \approx kA(t^*)\\
\]    
\[    A(t + \Delta t) \approx A(t) + k h A(t^*)\\ \]
    
\[    t = 0 \rightarrow A(\Delta t) \approx A(0) + k \Delta t A(t^*)\\ \]
    
\[    A(\Delta t) \approx A_0 + k h A_0\\
\]

\textbf{Example:} another model
\[ 
    \begin{cases}
        \frac{dA}{dt} = kA\\
        A(0) = a_0\\
    \end{cases}
\]

We can then use a bunch of techniques for the approximation of the limit that we discuessed last semester. recall the \textit{forward, backwards, and central} difference quotients.\\


\textbf{Errors in Our Approximations}\\

\[|f'(\bar{x}) - D_+f(\bar{x})| \]
\[= |f'(\bar{x}) - \frac{f(\bar{x} + h) - f(\bar{x})}{h}|\]
\[f(\bar{x} + h) = f(\bar{x}) + f'(\bar{x}) (\bar{x} + h - \bar{x}) + \frac{1}{2}f''(\bar{x})(\bar{x} + h - \bar{x})^2 + ...\]
\[f(\bar{x}) + h f'(\bar{x}) + \frac{1}{2} h^2 f''(\bar{x}) + ... \]
\[= | f'(\bar{x}) - \frac{1}{h} (h f'(\bar{x}) + \frac{1}{2} f''(\zeta) h^2) \rightarrow |-\frac{1}{2} h f''(\zeta)| \]

This allows us to establish the relationship
\[|f'(\bar{x}) - D_+ f(\bar{x}) | \leq Ch \]


\textbf{Homework:} compute the error in
\[ |f'(\bar{x}) - D_- f(\bar{x})| \]

\noindent \underline{\hspace{3in}}\\

\textbf{January 12, 2024}\\

\textbf{Example:} $D_+ f(\bar{x}) = \frac{f(\bar{x} + h) - f(\bar{x})}{h} \approx f'(\bar{x})$

\[err = |f'(x) - \frac{f(\bar{x} + h) - f(\bar{x})}{h}|\]
\[= |f'(\bar{x}) - \frac{1}{h}(f(\bar{x}) + f'(\bar{x})h + \frac{1}{2}f''(\zeta)h^2) - f(\bar{x})|\]
\[|-\frac{1}{2} h f''(\zeta)| \leq ch'\]


The idea above is called a \textbf{local truncatoin error analysis}.\\
\textbf{Implication:} To use this difference quotient and have
\[err \leq Ch\]
\textbf{Theorem:} $f$ must be twice continous differentiable on some interval containing $\bar{x}$\\

\textbf{Example:}
\[D_0f(\bar{x}) = \frac{f(\bar{x} + h) - f(x - h)}{2h} \]
\[err = |f'(\bar{x}) - \frac{1}{2h}(f(\bar{x}) + hf'(\bar{x}) + \frac{1}{2}h^2f''(\bar{x}) + \frac{1}{6}h^3 f'''(\zeta_1)) - (f(\bar{x}) +hf'(\bar{x}) + \frac{1}{2} h^2f''(\bar{x}) - \frac{1}{6} h^3 f'''(\zeta_2)|\]
\[= |- \frac{1}{12}h^2(f'(\zeta_1) + f'(\zeta_2)| \]
\[= \frac{1}{12} h^2 |f'''(\theta)|\]
\[\leq Ch^2\]

where
\[C = C(f'''(\zeta_1) + f'''(\zeta_2))\]


Lets recap. We want to find 
\[f'(\bar{x}) = D_+ f(\bar{x}) = \frac{1}{h}f(\bar{x} + h) - \frac{1}{h} f(x)\]


\textbf{Example:} suppose $f'(\bar{x}) \approx a_{-1} f(\bar{x} - h) + a_0 f(\bar{x}) + a_1 f(\bar{x} + h)$

This means

\[f(\bar{x} h) = f(\bar{x}) + f'(\bar{x})(\bar{x} - h - \bar{x}) + \frac{1}{2}f''(\bar{x}) (\bar{x} -h - \bar{x})^2 + \frac{1}{6} f'''(\zeta_1)(\bar{x} - h - \bar{x})^3\]
\[f(\bar{x}) = f(\bar{x})\]
\[f(\bar{x} + h) = f(\bar{x}) + f'(\bar{x})h + \frac{1}{2}f''(\bar{x})h^2 + \frac{1}{6}f'''(\zeta_2) h^3\]
\[f'(\bar{x}) = a_0(f(\bar{x}) + f'(\bar{x})h + \frac{1}{2}f''(\bar{x})h^2 + \frac{1}{6}f'''(\zeta_2) h^3) + a_0 f(\bar{x}) + a_1(f(\bar{x}) + f'(\bar{x})h + \frac{1}{2}f''(\bar{x})h^2 + \frac{1}{6}f'''(\zeta_2) h^3)\]
\[= f(\bar{x})(a_{-1} + a_0 + a_1) + h f'(\bar{x}) (-a_{-1} + a_1) + \frac{1}{2}h^2f''(\bar{x}) (a_{-1} + a_0) + \frac{1}{6} (f'''(\zeta_1) + f'''(\zeta_2))h^3\]

now, let
\[a_{-1} + a_0 + a_1 = 0\]
\[h(-a_{-1} + a_1) = 1\]
\[h^2(a_{-1} + a_1) = 0 \rightarrow a_{-1} + a_1 = 0\]

We can now use this system of equations to find $h$

\[a_{-1} = - a_1\]
\[h(a_1 + a_1) = 2h a_1 = 1 \rightarrow a_1 = \frac{1}{2h}\]
\[a_{-1} = -\frac{1}{2h}\]
\[a_0 = 0\]

We can now put this all together

\[f'(\bar{x}) = -\frac{1}{2h} f(\bar{x} - h) + \frac{1}{2h}f(\bar{x} + h)\]

And we get back the \textbf{central difference theorem} (amazin').\\

\textbf{Example:} 
$
\begin{cases}
    \frac{dA}{dt} = A(t)\\
    A(0) = A_0\\
\end{cases}\\
$
\[\frac{dA}{dt} \approx \frac{A(t + h) - A(t - h)}{2h}\]


\textbf{Example:} Define a function at a set of distributed points $x_1, x_2, ... x_n$ with the idea of approximating $u'(x)$ using
\[\bar{u}'(\bar{x}) = c_1 u(x_1) + c_2u(x_2) + ... + c_n(x_n)\]
\[|u'(x) - \sum_{k=1}^n c_k u(x_k)| \leq Ch^p\]
\[u(x_i) = u(\bar{x}) + u'(\bar{x}) (x_i - \bar{x}) + \frac{1}{2} u''(\bar{x})(x_i - \bar{x})^2 + ...\]
\[= \sum_{k=0}^n \frac{u^{(k)}(\bar{x})}{h!} (x_i - \bar{x})^2\]


\noindent \underline{\hspace{3in}}\\

\textbf{January 17, 2024}\\

\textbf{Topic:} Errors\\

\textbf{Example:} $d\hat{u}/dt = f(\hat{u}(t)); \hat{u}(0) = n \in \R$

Find all $u(t)$ that approximates $\hat{u}(t)$, try F.D.\\

\[d\hat{u}/dt = \frac{\hat{u}(t + h) - \hat{u}(t)}{h}\]
\[
    \begin{cases}
        \frac{\hat{u}(t + h) - \hat{u}(t)}{h} \approx f(\hat{u}(t))\\
         \hat{u}(0) = n
     \end{cases}
\]
\[\hat{u}(t + h) \approx \hat{u}(t) + hf(\hat{u}(t)\]

Define an approximation, u(t), by

\[\frac{u(t + h) - u(t)}{h} f(u(t))\]
\[u(t + h) = u(t) + hf(u(t))\]
\[u(0) = \mu \Rightarrow u(u + h) = u(0) + hf(u(0))\]

The error is defined as
\[E = \hat{u}(t) - u(t)\]
where $\hat{u}$ represents the approximation of $u$
A measure of the error
\[|E| = |\hat{u}(t) - u(t)| = abs.(E)\]

\textbf{Example:} $\hat{z} = 2.2, z = 2.20345$\\
\[E = 2.2 - 2.20345 = 0.00345 = |E|\]
Now, suppose $z$ and $\hat{z}$ are in terms of meters, and we decide to change from meters to nanometres
\[\hat{z} = 2.2 * 10^{9}, z = 2.20345 * 10^{9}, |E| = 0.00345 * 10^9 = 3.45 * 10^6 \]

Now, lets suppose we wanted to transform from meters into kilometers
\[\hat{z} = 2.2 * 10^{-3}, z = 2.20345 * 10^{-3}, |E| = 0.0345 * 10^{-3}\]
This example is \textit{poorly scaled}.\\

\textbf{Definition:} relative error
\[E_{|e|} = \frac{|\hat{z} - z|}{|\hat{z}|}\]
This gives us a \textit{dimensionless error}.\\

The problems we will work in will be assumed to be \textit{properly scaled}. This allows us to use the \textit{absolute error} ($E_{abs} = |E| = |\hat{z} - z|$)\\

\textbf{Definition:} Big-O notation\\

If $f(h)$ and $g(h)$ are functions of $h$, then 
\[f(h) = O(g(h))\]
as $h \to 0$ if
\[|\frac{f(h)}{g(h)}| \leq c; h\to0\]
or
\[|f(h)| \leq C|g(h)|\]

\textbf{Example:} $|D_+ f(\bar{x}) - f'(\bar{x})|$

\[= |f'(\bar{x}) - \frac{f(\bar{x} + h) - f(\bar{x})}{h}|\]
\[\leq |1/2 h f''(\zeta)|\]
\[\leq Ch\]
\[\Rightarrow |f'(\bar{x}) - D_+ f(\bar{x}) \leq Ch \]
\[\frac{|f'(\bar{x}) - D_+f(\bar{x})|}{h} \leq c\]
\[|f'(\bar{x}) - D_+f(\bar{x})| = O(h)\]

\textbf{Definition:} Little-o notation\\
For o(h)
\[f(h) = o(g(h)); \quad h \to 0\]
if
\[|\frac{f(h)}{g(h)}| \to 0\]
for $h$ sufficiently small.\\

\textbf{Example:} $2h^3 = O(h^2)$
\[2h^3 / h2 = 2h < c; \quad h < 1/c\]

\textbf{Example:} $2h^3 = o(h^2)$
\[2h^3 / h^2 = 2h \to 0; \quad h\to0\]

\textbf{Example:} $\sin(h) = O(h); \quad h\to 0$
\[\sin(h) = h - h^3/3! + h^5/5! ...; \quad h \in h\]
\[sin(h) < 1h = Ch \]

\textbf{Example:} $\sin(h) = h + O(h) \Rightarrow \sin(h) - h = O(h)$
\[(sin(h) - h)/h = O(n^3)\]

\textbf{Example:} $\sqrt{h} = O(1) \Rightarrow \sqrt{h} \to 0 < Ch$
\[\sqrt{h} = O(1) \to \sqrt{h} \ to 0 < Ch\]
\[\sqrt{h} = o(1) \ to \sqrt{h} \to 0\]
\[\sqrt{h} \neq O(h) \to \sqrt{h}/h \to 1/\sqrt{h}\]
\noindent \underline{\hspace{3in}}\\
\end{document}

